\documentclass[12pt]{article}

\input{../../preamble/defs.tex}
\input{../../preamble/envs.tex}
\input{../../preamble/packages.tex}

\title{Homework 2}
\author{Ryan Coyne}

\begin{document}
    \maketitle

    \begin{proof}{Let (\(G, \circ\)) be a group, and let \(g, h\in G\). Then 
        \begin{equation*}
            (g\circ h)^{-1} = h^{-1} \circ g^{-1}.
        \end{equation*}}
        First, we compose \((g \circ h)^{-1}\) with \((g\circ h)\). This gives us, \[(g \circ h)^{-1}\circ(g\circ h) = e.\] Next compose \(g^{-1}\circ h^{-1}\) with \((g\circ h)\). This gives us \begin{align*}
            (h^{-1}\circ g^{-1}) \circ (g\circ h) &= h^{-1} \circ (g^{-1} \circ g) \circ h\\
            & = h^{-1} \circ h\\
            & = e.
        \end{align*}
        Now, since \((g \circ h)^{-1}\circ(g\circ h) = (h^{-1}\circ g^{-1}) \circ (g\circ h)\), it follows that \((g \circ h)^{-1} = h^{-1}\circ g^{-1}\).
    \end{proof}
\end{document}